cp

theories/SLFStruct.v
@@ -34,95 +34,27 @@ Implicit Type L : list val.
     named [val_alloc] and [val_dealloc], for allocating and deallocating
     at once a range of consecutive memory cells.
 
-    For example, applying [val_alloc] to the integer value [3] would return
-    a pointer [p] together with the ownership of three cells: one at
-    location [p], one at location [p+1], and one atlocation [p+2].
+    In the first part of this chapter, we present the specification of
+    the operations on arrays and records. In the second part of this chapter,
+    we show how these operations can be implemented with heap of pointer
+    arithmetic operations, and specified with respect to a memory model
+    that exposes a particular representation of headers for allocated blocks.
 
-    This allocation model, which exposes pointer arithmetics, provides a way
-    to model both records and arrays with minimal extension to the semantics
-    of the programming language that we have considered sor far in the course.
-
-    The cells allocated using [val_alloc] are assigned as contents a special
-    value, named [val_uninit], to reflect for the fact that their contents has
-    never been set. Remark: in OCaml, one must provide an initialization
-    value explicitly, so there is no such thing as [val_uninit]; in JavaScript,
-    [val_uninit] is called [undefined]; in Java, arrays are initialized with
-    zeros; in C, uninitialized data should not be read---we could implement
-    this policy in our language by restricting the evaluation rule for the read
-    operation, adding a premise of the form [v <> val_uninit] to the rule.
-
-*)
-
-(* ########################################################### *)
-(** ** Updated source language *)
-
-(** The language is assumed to not include [val_ref] and [val_free],
-    but instead include primitive [val_alloc] and [val_dealloc] for
-    allocating blocks of cells.
-
-    The grammar of values is extended with two constructors:
-
-    - [val_uninit] describes the contents of an uninitialized cell.
-    - [val_header k] describes the contents of a header block for an
-      array or a record.
-
-*)
-
-Parameter val_uninit : val.
-Parameter val_header : nat -> val.
-
-Parameter val_uninit_neq_header :
-  forall k, val_uninit <> val_header k.
-(* Would be free if constructors were part of the inductive definition of [val] *)
-
-(** New primitive operations:
-
-    - [val_get_header p] to read a header, e.g., to get the length of an array,
-    - [val_alloc k] to allocate a block of [k] consecutive cells,
-    - [val_dealloc p] to deallocate the block at location [p].
-
-*)
-
-Parameter val_get_header : prim.
-Parameter val_alloc : prim.
-Parameter val_dealloc : prim.
-
-(** Semantics of allocation, deallocation, and reading of headers *)
-
-Parameter eval_alloc : forall k n ma mb p,
-  mb = Fmap.conseq (val_header k :: LibList.make k val_uninit) p ->
-  n = nat_to_Z k ->
-  p <> null ->
-  Fmap.disjoint ma mb ->
-  eval ma (val_alloc (val_int n)) (mb \+ ma) (val_loc p).
-
-Parameter eval_dealloc : forall k vs ma mb p,
-  mb = Fmap.conseq (val_header k :: vs) p ->
-  k = LibList.length vs ->
-  Fmap.disjoint ma mb ->
-  eval (mb \+ ma) (val_dealloc (val_loc p)) ma val_unit.
-
-Parameter eval_get_header : forall s p k,
-  Fmap.indom s p ->
-  (val_header k) = Fmap.read s p ->
-  eval s (val_get_header (val_loc p)) s (val_int k).
-
-Arguments eval_alloc : clear implicits.
-
-
-
-
+    This memory model is somewhat artificial, in the sense that it does not
+    perfectly match the memory model of an existing language----it is somewhere
+    between the memory model of C and that of OCaml. Nevertheless, this
+    memory model has the benefits of its simplicity, and it suffices to
+    illustrate formal proofs involving block headers and pointer arithmetics. *)
 
 
 (* ####################################################### *)
 (** ** Representation of a set of consecutive cells *)
 
-Module Cells.
+Module Specs.
 
-(** An array of length [k] allocated at location [p] can be represented
-    as a range of [k] consecutive cells starting from location [p]. In other
-    words, the array cells have addresses from [p] inclusive to [p+k]
-    exclusive.
+(** The cells from an array of length [k] can be represented as a range of [k]
+    consecutive cells, starting at some location [p]. In other words, the
+    array cells have addresses from [p] inclusive to [p+k] exclusive.
 
     The contents of an array of length [k] can be represented by a list
     of values of length [k]. This idea is formalized by the predicate [hcells].
@@ -143,11 +75,10 @@ Fixpoint hcells (L:list val) (p:loc) : hprop :=
   | x::L' => (p ~~> x) \* (hcells L' (S p))
   end.
 
-
 (** The description of an array, that is, a set of consecutive cells,
     can be split in two parts, at an arbitrary index. Concretely, if
     we have [harray (L1++L2) p], then we can separate the left part
-    [harray L1 p] from the right   part [harray L2 q], where the address
+    [harray L1 p] from the right part [harray L2 q], where the address
     [q] is equal to [p + length L1]. Reciprocally, the two parts can
     be merged back into the original form at any time. *)
 
@@ -157,94 +88,78 @@ Parameter hcells_concat_eq : forall p L1 L2,
 (** This "splitting lemma for arrays" is useful to carry out local
     reasoning on arrays, by focusing on the segment of the array involved
     in each recursive call, and obtaining for free the fact that the
-    cells outside of the segment remain unmodified.
-
-    The proof of the splitting lemma appears appears in the bonus section
-    of this chapter. *)
-
-(*
-Definition vals : Type := list val.
-*)
-
-Parameter hcells_focus : forall k p L,
-  k < length L ->
-  hcells L p ==>
-       ((p+k)%nat ~~> LibList.nth k L)
-    \* (\forall w, ((p+k)%nat ~~> w) \-* hcells (LibList.update k w L) p).
-
-
-(** Given a heap predicate [hcells L p], one can deduce that [p] is not
-    null, but only if the list [L] is not empty. In order to avoid in
-    proofs the need to treat specially the case empty arrays, it is
-    convenient to pack together with [hcells L p] the fact [p] is not null,
-    reflecting the fact that no data can be allocated at the null location,
-    not even an empty array.
-
-    The heap predicate [harray L p] packs together [hcells L p] with the
-    information [p <> null].
-*)
-
-Parameter hheader : forall (k:nat) (p:loc), hprop.
-
-Definition harray (L:list val) (p:loc) : hprop :=
-  hheader (length L) p \* hcells L (S p).
-
-Parameter harray_not_null : forall p L,
-  harray L p ==> harray L p \* \[p <> null].
+    cells outside of the segment remain unmodified. *)
 
 
 (* ####################################################### *)
-(** ** Specification of the allocation of consecutive cells *)
+(** ** Representation of an array with a block header *)
 
-(** The operation [val_alloc k] allocates [k] consecutive cells. Let [p]
-    denote the pointer returned. The allocated cells have addresses in
-    the range from [p] inclusive to [p+k] exclusive. These cells have for
-    contents is the special value [val_uninit], which we assume to be part
-    of the grammar of values. *)
+(** An array consists of a "header", and of the description of its cells.
+    The header is a heap predicate that describes the length of the array.
 
-(** The heap produced by [val_alloc k] can be described by [harray L p],
-    for a list [L] that consists of [k] occurences of the value [val_uninit].
-    Such a list is formally described by [LibList.make k val_uninit].
+    - In OCaml, the header consists of a physical memory cell at the
+      head of the array. This cell may be queried to obtain the length
+      of the array.
+    - In C, the header is a logical notion. It describes the length of
+      the allocated block, and it used in Separation Logic to specify
+      the behavior of the deallocation function, which can only be called
+      on the address of an allocated block, deallocating the full block
+      at once.
 
-    We introduce the heap predicate [harray_uninit k p] to denote the
-    specialization of [harray] to that list [LibList.make k val_uninit]. *)
+   In this course, we follow the OCaml view, with phyiscal headers.
+   However, the definitions could be easily adapted to follow the C view.
 
-Definition harray_uninit (k:nat) (p:loc) : hprop :=
-  harray (LibList.make k val_uninit) p.
+   The predicate [hheader k p] asserts the existence of an allocated
+   block at location [p], such that the contents of the block is made
+   of [k] cells (not counting the header cell). For the moment, we leave
+   its definition abstract. *)
 
-(** Let us specify the behavior of the allocation function using a
-    triple. We first state a specification with an argument of type [nat],
-    then reformulate the specification with an argument of type [int].
+Parameter hheader : forall (k:nat) (p:loc), hprop.
 
-    Consider a natural number [k]. Thanks to coercions, it may also be
-    viewed as an integer value of type [val].
+(** An array is described by the predicate [harray L p], where the list
+    [L] describes the contents of the cells. This heap predicate covers
+    both the header, which describes a block of length equal to [length L],
+    and the contents of the cells, described by [hcells L (p+1)].
+    Indeed, [p+1] is the first cell of the array, located next to the
+    header cell at location [p]. *)
 
-    The operation [val_alloc k] admits an empty precondition. Its
-    postcondition asserts that the return value [r] is of the form
-    [val_loc p] for some location [p], and that the final state
-    satisfies the heap predicate [harray_uninit k p]. Recall that this
-    predicate describes [k] cells at consecutive addresses starting from
-    location [p], with uninitialized contents. *)
+Definition harray (L:list val) (p:loc) : hprop :=
+  hheader (length L) p \* hcells L (p+1).
+
+
+(* ####################################################### *)
+(** ** Specification of allocation *)
+
+(** The primitive operation [val_alloc k] allocates a block made of
+    [k] consecutive cells. *)
+
+Parameter val_alloc : prim.
+
+(** The operation [val_alloc k] is specified as producing an array
+    whose cells contain the special "uninitialized value", written
+    [val_uninit]. *)
+
+Parameter val_uninit : val.
+
+(** More precisely, the postcondition of [val_alloc k] is of the form
+   [funloc p => harray L p], where the list [L] is defined as the
+   repetition of [k] times the value [val_uninit]. *)
 
 Parameter triple_alloc_nat : forall k,
   triple (val_alloc k)
     \[]
-    (funloc p => harray_uninit k p).
+    (funloc p => harray (LibList.make k val_uninit) p).
 
-(** We next generalize this specification so that it can handle applications
-    of the form [val_alloc n], where [n] is a nonnegative integer. Such a
-    presentation avoids the need to exhibit the natural number that corresponds
-    to the value [n].
-
-    The new specification, shown below, features the premise [n >= 0]. Its
-    postcondition involves the predicate [hcells (abs n) p], where [abs]
-    converts a nonnegative [int] value into the corresponding [nat] value. *)
+(** In practice, the operation [val_alloc] is applied to a non-negative
+    integer, that may not necessarily be syntactically a natural number.
+    Hence, the following lemma, which specifies [val_alloc n] for [n >= 0],
+    is more handy to use. *)
 
 Lemma triple_alloc : forall n,
   n >= 0 ->
   triple (val_alloc n)
     \[]
-    (funloc p => harray_uninit (abs n) p).
+    (funloc p => harray (LibList.make (abs n) val_uninit) p).
 Proof using.
   introv N. rewrite <- (@abs_nonneg n) at 1; [|auto].
   xtriple. xapp triple_alloc_nat. xsimpl*.
@@ -268,37 +183,28 @@ Qed.
 
 
 (* ####################################################### *)
-(** ** Specification of the deallocation of consecutive cells *)
+(** ** Specification of the deallocation *)
 
-(** The deallocation operation [val_dealloc n p] deallocates [n]
-    consecutive cells starting from the location [p]. It admits the
-    precondition [harray L p], where [L] can be any list of length [n],
-    and its postcondition is empty. *)
+(** The deallocation operation [val_dealloc p] deallocates the block
+    allocated at location [p]. *)
+
+Parameter val_dealloc : prim.
+
+(** The specification of [val_dealloc p] features a precondition that
+    requires an array of the form [harray L p], and an empty postcondition. *)
 
 Parameter triple_dealloc : forall L p,
   triple (val_dealloc p)
     (harray L p)
     (fun _ => \[]).
 
-(** Remark: in the C programming language, the argument [n] needs not be
-    provided, because the system keeps track of the size of allocated blocks.
-    One aspect that our simple semantics does not take into account is that
-    in C one can invoke the deallocation function only on pointers that were
-    produced by the allocation function. Extensions to the heap model and to
-    the Separation Logic can be devised to enforce this policy, yet they are
-    beyond the scope of this course. *)
-
-(** In the specification of deallocation presented above, the precondition
-    [harray L p] is stronger than it needs to be. Indeed, it would suffices
-    to require [hcells L p] in the precondition. Depending on the use case,
-    it may be easier for the user to not carry around the fact [p <> null],
-    which is embedded with [harray L p]. *)
+(** Observe that the [harray L p] predicate includes a header of the form
+    [hheader k p], ensuring that the corresponding allocated block is
+    deallocated exactly once. *)
 
 
 (* ####################################################### *)
 (** ** Specification of array operations *)
-
-Module Arrays.
 
 (** The operation [val_array_get p i] returns the contents of the [i]-th
     cell of the array at location [p]. *)
@@ -334,23 +240,31 @@ Parameter triple_array_set : forall L p i v,
     (harray L p)
     (fun _ => harray (LibList.update (abs i) v L) p).
 
-Hint Resolve triple_array_get triple_array_set : triple.
-
-(** Array length *)
+(** The operation [val_array_length p] returns the length of the array
+    allocated at location [p]. *)
 
 Parameter val_array_length : val.
+
+(** There are two useful specifications for [val_array_length]. The first
+    one operates with the heap predicate [harray L p]. The return value is
+    then the length of the list [L]. *)
 
 Parameter triple_array_length : forall L p,
   triple (val_array_length p)
     (harray L p)
     (fun r => \[r = length L] \* harray L p).
 
+(** The second specification for [val_array_length] operates only on the
+    header of the array. This small-footprint specification is useful to
+    read the length of an array whose cells are described by separated
+    segments, that is, after [hcells_concat_eq] has been exploited. *)
+
 Parameter triple_array_length_header : forall k p,
   triple (val_array_length p)
     (hheader k p)
     (fun r => \[r = (k:int)] \* hheader k p).
 
-End Arrays.
+Hint Resolve triple_array_get triple_array_set triple_array_length : triple.
 
 
 (* ########################################################### *)
@@ -415,6 +329,7 @@ Proof using. intros. math_rewrite (k+p = p+k)%nat. auto. Qed.
 Global Opaque hfield.
 
 
+End Specs.
 
 (* ########################################################### *)
 (** ** Allocation and deallocation of record fields *)
@@ -780,9 +695,9 @@ Qed.
 
 
 Lemma xapp_set_field_lemma : forall H k p v Q,
-  H ==> \exists kvs, (p ~~~> kvs) \* 
+  H ==> \exists kvs, (p ~~~> kvs) \*
      match hfields_update k v kvs with
-     | None => \[False] 
+     | None => \[False]
      | Some kvs' => ((fun _ => p ~~~> kvs') \--* protect Q) end ->
   H ==> wp (val_set_field k p v) Q.
 Proof using.
@@ -793,9 +708,9 @@ Proof using.
 Qed.
 
 Lemma xapp_get_field_lemma : forall H k p Q,
-  H ==> \exists kvs, (p ~~~> kvs) \* 
+  H ==> \exists kvs, (p ~~~> kvs) \*
      match hfields_lookup k kvs with
-     | None => \[False] 
+     | None => \[False]
      | Some v => ((fun r => \[r = v] \* p ~~~> kvs) \--* protect Q) end ->
   H ==> wp (val_get_field k p) Q.
 Proof using.
@@ -805,48 +720,10 @@ Proof using.
   { xpull. }
 Qed.
 
-
-Tactic Notation "xapp_nosubst" constr(E) :=
-  xseq_xlet_if_needed; xstruct_if_needed;
-  forwards_nounfold_then E ltac:(fun K => applys xapp_lemma K; xapp_simpl).
-  (* if [E] were already an instantiated lemma, then it would suffices
-     to call [applys xapp_lemma E; xapp_simpl]. But in the general case,
-     we need to instantiate [E] using the TLC tactic [forward_then] *)
-
-Tactic Notation "xapp_apply_spec" := (* internal *)
-  (* finds out the specification triple, from the hint data base [triple]
-     or in the context by looking for an induction hypothesis.
-     DISCLAIMER (explained in SLFWPgen): this approach does not work
-     for specifications that feature a premise that [eauto] cannot solve. *)
-  first [ solve [ eauto with triple ]
-        | match goal with H: _ |- _ => eapply H end ].
-
-Tactic Notation "xapp_nosubst" :=
-  xseq_xlet_if_needed; xstruct_if_needed;
-  first [ applys xapp_lemma; [ xapp_apply_spec | xapp_simpl ]
-        | applys xapp_set_field_lemma; xsimpl; simpl; xapp_simpl
+Ltac xapp_nosubst_for_records tt ::=
+  first [ applys xapp_set_field_lemma; xsimpl; simpl; xapp_simpl
         | applys xapp_get_field_lemma; xsimpl; simpl; xapp_simpl ].
 
-(** [xapp_try_subst] checks if the goal is of the form:
-    - either [forall (r:val), (r = ...) -> ...]
-    - or [forall (r:val), forall x, (r = ...) -> ...]
-
-    in which case it substitutes [r] away.
-*)
-
-Tactic Notation "xapp_try_subst" := (* internal *)
-  try match goal with
-  | |- forall (r:val), (r = _) -> _ => intros ? ->
-  | |- forall (r:val), forall x, (r = _) -> _ =>
-      let y := fresh x in intros ? y ->; revert y
-  end.
-
-Tactic Notation "xapp" constr(E) :=
-  xapp_nosubst E; xapp_try_subst.
-
-
-Tactic Notation "xapp" :=
-  xapp_nosubst; xapp_try_subst.
 
 Lemma triple_alloc_mcell' :
   triple (val_alloc 2%nat)
@@ -868,6 +745,91 @@ End GroupedFields.
 (* ########################################################### *)
 (* ########################################################### *)
 (** * Additional contents *)
+
+
+(* ########################################################### *)
+(** ** Updated source language *)
+
+
+    For example, applying [val_alloc] to the integer value [3] would return
+    a pointer [p] together with the ownership of three cells: one at
+    location [p], one at location [p+1], and one atlocation [p+2].
+
+    This allocation model, which exposes pointer arithmetics, provides a way
+    to model both records and arrays with minimal extension to the semantics
+    of the programming language that we have considered sor far in the course.
+
+    The cells allocated using [val_alloc] are assigned as contents a special
+    value, named [val_uninit], to reflect for the fact that their contents has
+    never been set. Remark: in OCaml, one must provide an initialization
+    value explicitly, so there is no such thing as [val_uninit]; in JavaScript,
+    [val_uninit] is called [undefined]; in Java, arrays are initialized with
+    zeros; in C, uninitialized data should not be read---we could implement
+    this policy in our language by restricting the evaluation rule for the read
+    operation, adding a premise of the form [v <> val_uninit] to the rule.
+
+
+(** The language is assumed to not include [val_ref] and [val_free],
+    but instead include primitive [val_alloc] and [val_dealloc] for
+    allocating blocks of cells.
+
+    The grammar of values is extended with two constructors:
+
+    - [val_uninit] describes the contents of an uninitialized cell.
+    - [val_header k] describes the contents of a header block for an
+      array or a record.
+
+*)
+
+Parameter val_uninit : val.
+Parameter val_header : nat -> val.
+
+Parameter val_uninit_neq_header :
+  forall k, val_uninit <> val_header k.
+(* Would be free if constructors were part of the inductive definition of [val] *)
+
+(** New primitive operations:
+
+    - [val_get_header p] to read a header, e.g., to get the length of an array,
+    - [val_alloc k] to allocate a block of [k] consecutive cells,
+    - [val_dealloc p] to deallocate the block at location [p].
+
+*)
+
+Parameter val_get_header : prim.
+Parameter val_alloc : prim.
+Parameter val_dealloc : prim.
+
+(** Semantics of allocation, deallocation, and reading of headers *)
+
+Parameter eval_alloc : forall k n ma mb p,
+  mb = Fmap.conseq (val_header k :: LibList.make k val_uninit) p ->
+  n = nat_to_Z k ->
+  p <> null ->
+  Fmap.disjoint ma mb ->
+  eval ma (val_alloc (val_int n)) (mb \+ ma) (val_loc p).
+
+Parameter eval_dealloc : forall k vs ma mb p,
+  mb = Fmap.conseq (val_header k :: vs) p ->
+  k = LibList.length vs ->
+  Fmap.disjoint ma mb ->
+  eval (mb \+ ma) (val_dealloc (val_loc p)) ma val_unit.
+
+Parameter eval_get_header : forall s p k,
+  Fmap.indom s p ->
+  (val_header k) = Fmap.read s p ->
+  eval s (val_get_header (val_loc p)) s (val_int k).
+
+Arguments eval_alloc : clear implicits.
+
+
+
+Definition hheader (k:nat) (p:loc) : hprop :=
+  fun h => (h = Fmap.single p (val_header k)) /\ (p <> null).
+
+Parameter harray_not_null : forall p L,
+  harray L p ==> harray L p \* \[p <> null].
+
 
 (* ####################################################### *)
 (** ** Allocation of records: example of list cells *)
@@ -930,7 +892,7 @@ Lemma triple_mcell : forall x q,
     (funloc p => p ~~~> `{ head := x ; tail := q }).
 Proof using.
   xwp. xapp triple_alloc_mcell'. intros p. xapp. xapp. xval. xsimpl*.
-Qed. 
+Qed.
 
 (** The function [mcons] is an alias for [mcell]. Whereas [mcell x q]
     is intended to allocate a fresh cell on its own, [mcons x q] is
@@ -1470,6 +1432,21 @@ Proof using.
   intros. unfold harray, null, loc. rewrite hcells_concat_eq.
   applys himpl_antisym; xsimpl*. math.
 Qed.
+
+
+
+(* ########################################################### *)
+(** ** Focus lemma *)
+
+(** Another useful lemma
+
+Parameter hcells_focus : forall k p L,
+  k < length L ->
+  hcells L p ==>
+       ((p+k)%nat ~~> LibList.nth k L)
+    \* (\forall w, ((p+k)%nat ~~> w) \-* hcells (LibList.update k w L) p).
+
+
 
 
 (* ########################################################### *)
